\maketitle
Here are some mathematical equations that are used when finite elements are to be calculated:

\begin{equation}
    \dot{q_1} = {\frac{k}{L}}(T_1-T_2)
\end{equation}
\begin{equation}
    \dot{q_2} = -{\frac{k}{L}}(T_1-T_2)
\end{equation}
\begin{equation}
    \dot{\bar{q_2^e}} = \dot{\bar{k^e}}\cdot\dot{\bar{T^e}}
\end{equation}

\begin{equation}
    \bar{k}^e = 
    \begin{bmatrix}
        k_{11}^e & k_{12}^e \\
        k_{21}^e & k_{22}^e
    \end{bmatrix}
     = \frac{k}{L}
     \begin{bmatrix}
         1 & -1 \\
         -1 & 1
     \end{bmatrix}
\end{equation}

\begin{equation}
\dot{\bar{T^e}} = 
    \begin{Bmatrix}
    T_1 \\ T_2
    \end{Bmatrix}
\end{equation}

\begin{equation}
\dot{\bar{q^e}} = 
    \begin{Bmatrix}
    q_1 \\ q_2
    \end{Bmatrix}
\end{equation}

\begin{equation}
    \bar{c^e} = \frac{L \cdot c \cdot \rho}{2}
    \begin{bmatrix}
        1 & 0 \\ 0 & 1
    \end{bmatrix}
\end{equation}

\begin{equation}
    \bar{K} = 
    \begin{bmatrix}
        k_{11}^1 & k_{12}^1 & 0 & 0 \\
        k_{12}^1 & (k_{22}^1 + k_{11}^2) & k_{12}^2 & 0 \\
        0 & k_{21}^2 & (k_{22}^2 + k_{11}^3) & k_{12}^3 \\
        0 & 0 & k_{21}^3 & k_{22}^3
    \end{bmatrix}
\end{equation}

\begin{equation}
    \bar{C} \cdot \dot{\bar{T}} + \bar{K} \cdot \bar{T} = \bar{Q}
\end{equation}

\begin{equation}
    \dot{Q_i} = 
    \epsilon \sigma (T^4_r - T^4_{s,i}) + h(T_g - T_{s,i})
\end{equation}

\begin{equation}
    \bar{\dot{T}} \cong \frac{\Delta\bar{T}}{\Delta t} = 
    \frac{\bar{T}^{j+1} - \bar{T}^j}{\Delta t}
\end{equation}

\begin{equation}
    \bar{C} = 
    \begin{bmatrix}
        \frac{\bar{T}^{j+1} - T^j}{\delta t}
    \end{bmatrix}
    + \bar{K}\bar{T} = \bar{Q}
\end{equation}

\begin{equation}
    \bar{T}^{j+1} = 
    \begin{pmatrix}
    \frac{\bar{C}}{\Delta t} + \bar{K}
    \end{pmatrix}^{-1}
    \cdot
    \begin{pmatrix}
    \bar{Q}^j + \bar{C}\bar{T}^j
    \end{pmatrix} \Delta t
\end{equation}